Update etc/ci-goose-check; regoose

etc/ci-goose-check.py
@@ -34,6 +34,7 @@ projs = {
     "gokv": Proj.make("gokv", "https://github.com/mit-pdos/gokv", commit="upamanyus-fixes"),
     "etcd-raft": Proj.make("etcd-raft", "https://github.com/upamanyus/etcd-raft"),
     "etcd": Proj.make("etcd", "https://github.com/upamanyus/etcd"),
+    "go-journal": Proj.make("etcd", "https://github.com/mit-pdos/go-journal"),
 }
 
 
@@ -108,6 +109,8 @@ def main():
             projs["etcd"].path(),
             "--etcd-raft",
             projs["etcd-raft"].path(),
+            "--go-journal",
+            projs["go-journal"].path(),
         ],
         check=True,
     )
